Here are some examples of questions and solutions followed by a new question that you need to solve.
Make sure to put the answer (and only answer) inside \boxed{{}}.



Question:
A parabola with equation $y=x^2+bx+c$ passes through the points $(-1,-11)$ and $(3,17)$. What is $c$? 


My solution:
From the question we know that points $(-1, -11)$ and $(3, 17)$ lie on the parabola. This means that when we substitute $x$ and $y$ from these points into the equation $y = x^2 + bx + c$, the equation must hold true. We substitute these two points into the given equation to solve for $c$.

For the point $(-1, -11)$:

Substitute $x = -1$ and $ y = -11 $ into the equation:
\[ -11 = (-1)^2 + b(-1) + c \Rightarrow -11 = 1 - b + c \Rightarrow -b + c = -12 \]

For the point $(3, 17)$:

Substitute $x = 3$ and $y = 17$ into the equation:
\[ 17 = (3)^2 + b(3) + c \Rightarrow 17 = 9 + 3b + c \Rightarrow 3b + c = 8 \]

In summary, we have the two equations
\begin{align*}
-b + c &= -12\\
3b + c &= 8
\end{align*}

To solve for $c$ we can eliminate $b$ by multiplying the first equation by 3 and adding equations together.
Multiplying the first equation by 3, we have $3(-b + c) = 3 (-12) \Rightarrow -3b + 3c = -36$. Adding equations together gives us
\[ (-3b + 3c) + (3b + c) = -36 + 8 \Rightarrow -3b + 3b + 3c + c = -28 \Rightarrow 4c = -28 \Rightarrow c = -28 : 4 \Rightarrow c = \boxed{-7} \]






Question:
Let $f(x)$ be an odd function.  Is $f(f(x))$ even, odd, or neither?\n\nEnter "odd", "even", or "neither".


My solution:
To determine whether $f(f(x))$ is even, odd, or neither, we need to use the property of $f(x)$ being an odd function.

An odd function is defined as:
\[ f(-x) = -f(x) \quad \text{for all } x \]

Given that $f(x)$ is odd, let's find $f(f(-x))$ and see how it relates to $f(f(x))$.

1. Substitute $-x$ into the function $f(x)$:
\[ f(-x) \]

2. Since $f(x)$ is odd, apply the definition of an odd function:
\[ f(-x) = -f(x) \]

3. Now substitute $-f(x)$ into the function $f$:
\[ f(f(-x)) = f(-f(x)) \]

4. Again, using the fact that $f(x)$ is odd, apply the definition:
\[ f(-f(x)) = -f(f(x)) \]

5. We have found that:
\[ f(f(-x)) = -f(f(x)) \]

This matches the definition of an odd function.

So, the answer is:
\[ \boxed{\text{odd}} \]






Question:
A rectangular box $P$ is inscribed in a sphere of radius $r$. The surface area of $P$ is 384, and the sum of the lengths of its 12 edges is 112. What is $r$?


My solution:
Let the dimensions of the rectangular box $P$ be $x$, $y$, and $z$. We know the following:

1. The sum of the lengths of the edges of $P$ is
\[ 4(x + y + z) = 112 \Rightarrow x + y + z = 112 : 4 \Rightarrow x + y + z = 28 \]

2. The surface area of $P$ is
\[ 2xy + 2yz + 2xz = 384 \Rightarrow xy + yz + xz = 384 : 2 \Rightarrow xy + yz + xz = 192 \]

Since the box is inscribed in the sphere, the diagonal of the box is the diameter of the sphere. The length of the diagonal is $\sqrt{x^2 + y^2 + z^2}$

The diameter of the sphere is $2r$, so:
\[ 2r = \sqrt{x^2 + y^2 + z^2} \Rightarrow (2r)^2 = x^2 + y^2 + z^2 = (x + y + z)^2 - (2xy + 2yz + 2xz) \]

Substitute the known values:
\[ 4r^2 = 28^2 - 384 = 784 - 384 = 400 \Rightarrow r^2 = 100 \Rightarrow r = \boxed{10} \]






Question:
Let $\mathbf{a} = \begin{pmatrix} 2 \\ 1 \\ 5 \end{pmatrix}.$  Find the vector $\mathbf{b}$ such that $\mathbf{a} \cdot \mathbf{b} = 11$ and\n\[\mathbf{a} \times \mathbf{b} = \begin{pmatrix} -13 \\ -9 \\ 7 \end{pmatrix}.\]


My solution:
Let $\mathbf{b} = \begin{pmatrix} x \\ y \\ z \end{pmatrix}$.

First, use the dot product condition:
\[ \mathbf{a} \cdot \mathbf{b} = 11 \Rightarrow 2x + y + 5z = 11 \]

Next, use the cross product condition:
\[ \mathbf{a} \times \mathbf{b} = \begin{pmatrix} 2 \\ 1 \\ 5 \end{pmatrix} \times \begin{pmatrix} x \\ y \\ z \end{pmatrix} = \begin{pmatrix} -5y + z \\ 5x - 2z \\ -x + 2y \end{pmatrix} = \begin{pmatrix} -13 \\ -9 \\ 7 \end{pmatrix} \]

This gives us the system of equations:
   \begin{align*}
   2x + y + 5z = 11 \quad &(1) \\
   -5y + z = -13 \quad &(2) \\
   5x - 2z = -9 \quad &(3) \\
   -x + 2y = 7 \quad &(4)
   \end{align*}

Solve for $x$, $y$, and $z$ step-by-step:

From (2), $z = 5y - 13$.
From (4), $x = 2y - 7$.

Substitute $z = 5y - 13$ into (1):
\[ 2(2y - 7) + y + 5(5y - 13) = 11 \Rightarrow 4y - 14 + y + 25y - 65 = 11 \Rightarrow 30y - 79 = 11 \Rightarrow 30y = 90 \Rightarrow y = 3 \]

Now find $x$ and $z$:
\[ x = 2y - 7 = 2(3) - 7 = -1 \]

\[ z = 5y - 13 = 5(3) - 13 = 2 \]

Thus, the vector $\mathbf{b}$ is:
\[ \mathbf{b} = \boxed{\begin{pmatrix} -1 \\ 3 \\ 2 \end{pmatrix}} \]






Question:
{question}



My solution: